assert and run.sh: update

asset/tmp/impl/rsl/Constants.i.dfy
@@ -58,8 +58,10 @@ module Impl_LiveRSL__Constants_i
 
 	function method CReplicaConstantsValid(c: CReplicaConstants) : bool 
 		requires CReplicaConstantsIsValid(c)
-		ensures CReplicaConstantsValid(c) == LReplicaConstantsValid(AbstractifyCReplicaConstantsToLReplicaConstants(c))
+		ensures var lr := LReplicaConstantsValid(AbstractifyCReplicaConstantsToLReplicaConstants(c)); var cr := CReplicaConstantsValid(c); (cr) == (lr)
 	{
-		HOLDER
+		0 <= c.my_index 
+		&& 
+		c.my_index < |c.all.config.replica_ids|
 	}
 }
