asset/tmp/impl/rsl/Election.i.dfy
@@ -1,1 +1,47 @@
-Error: TopLevel.find_module: not found: (Internal.NonEmptyList.:: ("LiveRSL__Election_i", []))
+include ""
+
+
+module Impl_LiveRSL__Election_i 
+{
+
+	datatype CElectionState = 
+	CElectionState(
+		constants: CReplicaConstants, 
+		current_view: CBallot, 
+		current_view_suspectors: set<int>, 
+		epoch_end_time: int, 
+		epoch_length: int, 
+		requests_received_this_epoch: seq<CRequest>, 
+		requests_received_prev_epochs: seq<CRequest>
+	)
+
+	predicate CElectionStateIsValid(s: CElectionState) 
+	{
+		CElectionStateIsAbstractable(s) 
+		&& 
+		CReplicaConstantsIsValid(s.constants) 
+		&& 
+		CBallotIsValid(s.current_view) 
+		&& 
+		(forall i :: i in s.requests_received_this_epoch ==> CRequestIsValid(i)) 
+		&& 
+		(forall i :: i in s.requests_received_prev_epochs ==> CRequestIsValid(i))
+	}
+
+	predicate CElectionStateIsAbstractable(s: CElectionState) 
+	{
+		CReplicaConstantsIsAbstractable(s.constants) 
+		&& 
+		CBallotIsAbstractable(s.current_view) 
+		&& 
+		(forall i :: i in s.requests_received_this_epoch ==> CRequestIsAbstractable(i)) 
+		&& 
+		(forall i :: i in s.requests_received_prev_epochs ==> CRequestIsAbstractable(i))
+	}
+
+	function AbstractifyCElectionStateToElectionState(s: CElectionState) : ElectionState 
+		requires CElectionStateIsAbstractable(s)
+	{
+		ElectionState(AbstractifyCReplicaConstantsToLReplicaConstants(s.constants), AbstractifyCBallotToBallot(s.current_view), s.current_view_suspectors, s.epoch_end_time, s.epoch_length, AbstractifySeq(s.requests_received_this_epoch, AbstractifyCRequestToRequest), AbstractifySeq(s.requests_received_prev_epochs, AbstractifyCRequestToRequest))
+	}
+}
