asset/tmp/impl/rsl/Proposer.i.dfy
@@ -1,1 +1,131 @@
-Error: TopLevel.find_module: not found: (Internal.NonEmptyList.:: ("LiveRSL__Proposer_i", []))
+include ""
+
+
+module Impl_LiveRSL__Proposer_i 
+{
+
+	datatype CIncompleteBatchTimer = 
+	CIncompleteBatchTimerOn(
+		when: int
+	)
+	 | 
+	CIncompleteBatchTimerOff(
+		
+	)
+
+	predicate CIncompleteBatchTimerIsValid(s: CIncompleteBatchTimer) 
+	{
+		match s
+		case CIncompleteBatchTimerOn(when) => CIncompleteBatchTimerIsAbstractable(s)
+		case CIncompleteBatchTimerOff() => CIncompleteBatchTimerIsAbstractable(s)
+
+	}
+
+	predicate CIncompleteBatchTimerIsAbstractable(s: CIncompleteBatchTimer) 
+	{
+		match s
+		case CIncompleteBatchTimerOn(when) => true
+		case CIncompleteBatchTimerOff() => true
+
+	}
+
+	function AbstractifyCIncompleteBatchTimerToIncompleteBatchTimer(s: CIncompleteBatchTimer) : IncompleteBatchTimer 
+		requires CIncompleteBatchTimerIsAbstractable(s)
+	{
+		match s
+		case CIncompleteBatchTimerOn(when) => IncompleteBatchTimerOn(s.when)
+		case CIncompleteBatchTimerOff() => IncompleteBatchTimerOff()
+
+	}
+
+	datatype CProposer = 
+	CProposer(
+		constants: CReplicaConstants, 
+		current_state: int, 
+		request_queue: seq<CRequest>, 
+		max_ballot_i_sent_1a: CBallot, 
+		next_operation_number_to_propose: int, 
+		received_1b_packets: set<CPacket>, 
+		highest_seqno_requested_by_client_this_view: map<EndPoint, int>, 
+		incomplete_batch_timer: CIncompleteBatchTimer, 
+		election_state: CElectionState
+	)
+
+	predicate CProposerIsValid(s: CProposer) 
+	{
+		CProposerIsAbstractable(s) 
+		&& 
+		CReplicaConstantsIsValid(s.constants) 
+		&& 
+		(forall i :: i in s.request_queue ==> CRequestIsValid(i)) 
+		&& 
+		CBallotIsValid(s.max_ballot_i_sent_1a) 
+		&& 
+		(forall i :: i in s.received_1b_packets ==> CPacketIsValid(i)) 
+		&& 
+		(forall i :: i in s.highest_seqno_requested_by_client_this_view ==> EndPointIsValid(i)) 
+		&& 
+		CIncompleteBatchTimerIsValid(s.incomplete_batch_timer) 
+		&& 
+		CElectionStateIsValid(s.election_state)
+	}
+
+	predicate CProposerIsAbstractable(s: CProposer) 
+	{
+		CReplicaConstantsIsAbstractable(s.constants) 
+		&& 
+		(forall i :: i in s.request_queue ==> CRequestIsAbstractable(i)) 
+		&& 
+		CBallotIsAbstractable(s.max_ballot_i_sent_1a) 
+		&& 
+		(forall i :: i in s.received_1b_packets ==> CPacketIsAbstractable(i)) 
+		&& 
+		(forall i :: i in s.highest_seqno_requested_by_client_this_view ==> EndPointIsAbstractable(i)) 
+		&& 
+		CIncompleteBatchTimerIsAbstractable(s.incomplete_batch_timer) 
+		&& 
+		CElectionStateIsAbstractable(s.election_state)
+	}
+
+	function AbstractifyCProposerToLProposer(s: CProposer) : LProposer 
+		requires CProposerIsAbstractable(s)
+	{
+		LProposer(AbstractifyCReplicaConstantsToLReplicaConstants(s.constants), s.current_state, AbstractifySeq(s.request_queue, AbstractifyCRequestToRequest), AbstractifyCBallotToBallot(s.max_ballot_i_sent_1a), s.next_operation_number_to_propose, AbstractifySet(s.received_1b_packets, AbstractifyCPacketToRslPacket), AbstractifyMap(s.highest_seqno_requested_by_client_this_view, AbstractifyEndPointToNodeIdentity, NoChange, AbstractifyNodeIdentityToEndPoint), AbstractifyCIncompleteBatchTimerToIncompleteBatchTimer(s.incomplete_batch_timer), AbstractifyCElectionStateToElectionState(s.election_state))
+	}
+
+	function method CProposerCheckForQuorumOfViewSuspicions(s: CProposer, clock: int) : CProposer 
+		requires CProposerIsValid(s)
+		ensures var s' := CProposerCheckForQuorumOfViewSuspicions(s, clock); CProposerIsValid(s') && LProposerCheckForQuorumOfViewSuspicions(AbstractifyCProposerToLProposer(s), AbstractifyCProposerToLProposer(s'), clock)
+	{
+		var t1 := 
+			CElectionStateCheckForQuorumOfViewSuspicions(s.election_state, clock); 		
+		var t2 := 
+			if CBalLt(s.election_state.current_view, t1.current_view) then 
+				var t1 := 
+					0; 				
+				var t2 := 
+					[]; 				
+				(t1, t2) 
+			else 
+				var t1 := 
+					s.current_state; 				
+				var t2 := 
+					s.request_queue; 				
+				(t1, t2); 		
+		var t3 := 
+			s.(election_state := t1, current_state := t2.1, request_queue := t2.0); 		
+		t3
+	}
+
+	function method CProposerResetViewTimerDueToExecution(s: CProposer, val: CRequestBatch) : CProposer 
+		requires CProposerIsValid(s)
+		requires CRequestBatchIsValid(val)
+		ensures var s' := CProposerResetViewTimerDueToExecution(s, val); CProposerIsValid(s') && LProposerResetViewTimerDueToExecution(AbstractifyCProposerToLProposer(s), AbstractifyCProposerToLProposer(s'), AbstractifyCRequestBatchToRequestBatch(val))
+	{
+		var t1 := 
+			CElectionStateReflectExecutedRequestBatch(s.election_state, val); 		
+		var t2 := 
+			s.(election_state := t1); 		
+		t2
+	}
+}
